

Using

$$\frac{dB}{dt} - \alpha B = -r \quad (1)$$

with initial conditions

$$B(0) = B_0 \quad \text{and} \quad B(T) = 0$$

where

- >  $B(t)$  is the outstanding mortgage balance at time  $t$
- >  $\alpha$  is the constant interest rate (per unit time)
- >  $r$  is the repayment rate (per unit time)

Constant interest rate

Solve using integrating factor method

$$\frac{dB}{dt} + P(t)B = Q(t)$$

rewrite as

$$\frac{dB}{dt} + (-\alpha)B = -r$$

$$\text{let } P(t) = -\alpha \quad \text{and} \quad Q(t) = -r$$

Our integrating factor is

$$\mu(t) = e^{\int P(t) dt} = e^{\int -\alpha dt} = e^{-\alpha t}$$

next multiply both sides of ODE by  $\mu(t) = e^{-\alpha t}$

$$e^{-\alpha t} \frac{dB}{dt} - \alpha e^{-\alpha t} B = -r e^{-\alpha t}$$

the L.H.S is derivative of  $B(t)e^{-\alpha t}$

$$\frac{d}{dt}(B(t)e^{-\alpha t}) = -r e^{-\alpha t}$$

$$\int \frac{d}{dt}(B(t)e^{-\alpha t}) dt = \int -r e^{-\alpha t} dt$$

$$B(t)e^{-\alpha t} = \int -r e^{-\alpha t} dt$$

Since  $r$  is const r.h.s is

$$\int -r e^{-\alpha t} dt = -r \int e^{-\alpha t} dt = -r \left( \frac{e^{-\alpha t}}{-\alpha} \right) = \frac{r}{\alpha} e^{-\alpha t}$$

add constant  $C$

$$B(t)e^{-\alpha t} = \frac{r}{\alpha} e^{-\alpha t} + C$$

multiply both sides by  $e^{\alpha t}$

$$B(t) = \frac{r}{\alpha} + C e^{\alpha t}$$

Apply initial condition  $B(0) = B_0$

$$B(0) = \frac{r}{\alpha} + C e^0 = \frac{r}{\alpha} + C = B_0$$

$$\Rightarrow C = B_0 - \frac{r}{\alpha}$$

So solution becomes

$$B(t) = \frac{r}{\alpha} + \left(B_0 - \frac{r}{\alpha}\right) e^{\alpha t} = B_0 e^{\alpha t} - \frac{r}{\alpha} (e^{\alpha t} - 1)$$

determining repayment rate  $r$  using  $B(T) = 0$   
mortgage is fully repaid at  $t = T$

$$B(T) = B_0 e^{\alpha T} - \frac{r}{\alpha} (e^{\alpha T} - 1) = 0$$

Solve for  $r$ :

$$B_0 e^{\alpha T} = \frac{r}{\alpha} (e^{\alpha T} - 1)$$

$$r = \frac{\alpha B_0 e^{\alpha T}}{e^{\alpha T} - 1}$$

### Variable interest rate solution

let  $\alpha = \alpha(t)$  and rewrite (1) as

$$\frac{dB}{dt} - \alpha(t) B = -r \quad (2)$$

1<sup>st</sup> order linear ODE

its of the form

$$\frac{dB}{dt} + P(t) B = Q(t)$$

integrating factor is  $M(t) = e^{\int P(t) dt}$

rewrite (2)

$$\frac{dB}{dt} + (-\alpha(t)) B = -r$$

so

$$P(t) = -\alpha(t)$$

$\therefore$

$$M(t) = e^{-\int_0^t \alpha(s) ds}$$

multiply by  $M(t)$

$$e^{-\int_0^t \alpha(s) ds} \frac{dB}{dt} - \alpha(t) e^{-\int_0^t \alpha(s) ds} B = -r e^{-\int_0^t \alpha(s) ds}$$

$$\frac{d}{dt} \left( B(t) e^{-\int_0^t \alpha(s) ds} \right) = -r e^{-\int_0^t \alpha(s) ds}$$

$$B(t) e^{-\int_0^t \alpha(s) ds} - B(0) = -r \int_0^t e^{-\int_0^u \alpha(s) ds} du$$

using  $B(0) = B_0$

$$B(t)e^{-\int_0^t \alpha(s) ds} = B_0 - r_0 \int_0^t e^{-\int_0^s \alpha(u) du} ds$$

multiply both sides by  $e^{\int_0^t \alpha(s) ds}$

$$B(t) = e^{\int_0^t \alpha(s) ds} \left[ B_0 - r_0 \int_0^t e^{-\int_0^s \alpha(u) du} ds \right]$$

Now  $B(T) = 0$

Sub  $t = T$

$$0 = e^{\int_0^T \alpha(s) ds} \left[ B_0 - r_0 \int_0^T e^{-\int_0^s \alpha(u) du} ds \right]$$

$$B_0 = r_0 \int_0^T e^{-\int_0^s \alpha(u) du} ds$$

rearrange

$$\int_0^T e^{-\int_0^s \alpha(u) du} ds = \frac{B_0}{r}$$